smt notations, but variable names containing ' cause trouble
because not allowed in smt and quoting them in |...| creates
conflicts between printing Zs and vars

LiveVerif/src/LiveVerifExamples/Tests/SampleSideconds.v
@@ -37,60 +37,319 @@ Ltac standalone_solver_step :=
       | solve [intuition idtac]
     ].
 
-Ltac t := repeat standalone_solver_step.
-
 (* TODO investigate why standalone_solver_step is not as powerful as step *)
 
-Load LiveVerif.
+Require Import Coq.Logic.Classical_Prop.
 
-Goal forall (b n : word) (bs : list Z),
- len bs = \[n] ->
- forall (i : word),
- \[b] < 2 ^ 8 -> i = /[0] -> List.repeatz \[b] \[i] ++ bs[\[i]:] = bs.
-Proof. t. Qed.
+Lemma ExistsNot_NotForall: forall AA (P: AA -> Prop), (exists a: AA, ~ P a) <-> ~ forall (a: AA), P a.
+Proof.
+  intros. split.
+  - intros. destruct H as [a H]. intro. apply H. auto.
+  - intro. destruct (classic (exists a : AA, ~ P a)) as [C | C]; [assumption|].
+    exfalso. apply H. intro. destruct (classic (P a)) as [D | D]; [assumption |].
+    exfalso. apply C. exists a. assumption.
+Qed.
+
+Inductive Name := mkName (f: unit -> unit).
+Notation "'name:(' x )" := (mkName (fun x: unit => x)) (format "name:( x )").
+
+Definition smtFalseAlias := False.
+Definition smtGoalMarker(P: Prop) := P.
+Definition namedSmtGoalMarker(width: Z)(n: Name)(P: Prop) := P.
+
+Ltac markSmtGoal :=
+  lazymatch goal with
+  | |- ?g => change (smtGoalMarker g)
+  end.
+
+Ltac markNamedSmtGoal width name :=
+  lazymatch goal with
+  | |- ?g => change (namedSmtGoalMarker width name g)
+  end.
+
+Ltac unmarkSmtGoal :=
+  lazymatch goal with
+  | |- smtGoalMarker ?g => change g
+  | |- namedSmtGoalMarker _ _ ?g => change g
+  end.
+
+(* turns
+     forall x1 ... xN, P
+   into
+     forall x1 ... xN, ~ P -> smtFalseAlias
+   where the xi can be (dependent) variables or (non-dependent) hypotheses in any order.
+   Also clears unused non-Prop variables. *)
+Ltac by_contradiction :=
+  eapply NNPP;
+  let C := fresh "C" in
+  intro C;
+  repeat lazymatch type of C with
+  | ~ forall H, _ =>
+      eapply ExistsNot_NotForall in C;
+      let name := fresh H in
+      destruct C as [name C]
+  end;
+  change smtFalseAlias;
+  repeat lazymatch goal with
+         | H: ?T |- _ => lazymatch T with
+                         | word.word _ => fail
+                         | @word.ok _ _ => fail
+                         | _ => lazymatch type of T with
+                                | Prop => revert H
+                                (* clear unused variables, because otherwise the notations
+                                   print it as an assert instead of declare-const *)
+                                | _ => clear H || revert H
+                                end
+                         end
+         end.
+
+Ltac undo_by_contradiction :=
+  intros;
+  lazymatch goal with
+  | C: not _ |- smtFalseAlias => apply C; clear C
+  end.
+
+Ltac log_goal_as_smt name :=
+  by_contradiction;
+  let width := lazymatch goal with
+               | word: word.word ?width |- _ => width
+               end in
+  (* markNamedSmtGoal width name; *)
+  markSmtGoal;
+  lazymatch goal with
+  | |- ?g => idtac g
+  end;
+  unmarkSmtGoal;
+  undo_by_contradiction.
+
+Declare Custom Entry smt_sort.
+Declare Custom Entry smt_expr.
+Declare Custom Entry smt_goal.
+Declare Custom Entry smt_func.
+
+(* Goal Structure: *)
+
+(* TODO conflicts with SuppressibleWarnings, probably better to not do this at all
+Notation "g" := (smtGoalMarker g)
+  (at level 100, g custom smt_goal at level 3, only printing). *)
+
+Notation "'(BEGIN' 'SMT' 'QUERY)' g '(END' 'SMT' 'QUERY)'" := (smtGoalMarker g)
+  (at level 10, g custom smt_goal at level 3,
+   format "(BEGIN  SMT  QUERY) '//' g '//' (END  SMT  QUERY)").
+
+(* bash syntax to print to a file *)
+Notation "'cat' > './width' W / x '.smt2' << ' 'SMTQUERY' ' g 'SMTQUERY'" :=
+  (namedSmtGoalMarker W (mkName (fun x => x)) g)
+  (at level 0, g custom smt_goal at level 3, only printing,
+   format "cat  >  ./width W / x .smt2  << ' SMTQUERY ' '//' g '//' SMTQUERY").
+
+(* bash syntax to print to feed to z3's stdin *)
+Notation "'time' 'z3' '-in' << ' 'SMTQUERY' ' g 'SMTQUERY'" :=
+  (smtGoalMarker g)
+  (at level 0, g custom smt_goal at level 3, only printing,
+   format "time  z3  -in  << ' SMTQUERY ' '//' g '//' SMTQUERY").
+
+Notation "'(declare-const' | x | T ) P" := (forall x: T, P)
+  (in custom smt_goal at level 3, x name, T custom smt_sort, right associativity,
+   format "(declare-const  | x |  T ) '//' P").
+
+(* TODO recursive notation for any number of parameters? *)
+Notation "'(declare-fun' | x | ( A1 ) R ) P" := (forall x: A1 -> R, P)
+  (in custom smt_goal at level 3, x name, A1 custom smt_sort, R custom smt_sort,
+   right associativity,
+   format "(declare-fun  | x |  ( A1 )  R ) '//' P").
+
+Notation "'(assert' P ) Q" := (P -> Q)
+  (in custom smt_goal at level 3, P custom smt_expr, right associativity,
+   format "(assert  P ) '//' Q").
+
+Notation "'(check-sat)'" := smtFalseAlias (in custom smt_goal).
+
+
+(* Sorts: *)
+
+Notation "'(_' 'BitVec' Width ')'" := (@word.rep Width _)
+  (in custom smt_sort, Width constr at level 0).
+Notation "'Int'" := Z
+  (in custom smt_sort).
+Notation "'Bool'" := bool
+  (in custom smt_sort, only printing).
+Notation "'Bool'" := Prop
+  (in custom smt_sort, only printing).
+(* hides Bool notations?
+Notation "x" := x
+  (in custom smt_sort at level 0, x constr at level 0). *)
+
+(* Expressions: *)
+
+Notation "( 'an' 'd' a b )" := (andb a b)
+  (in custom smt_expr at level 0, format "( an d  a  b )", only printing).
+Notation "( 'o' 'r' a b )" := (orb a b)
+  (in custom smt_expr at level 0, format "( o r  a  b )", only printing).
+Notation "( 'no' 't' P )" := (negb P)
+  (in custom smt_expr at level 0, format "( no t  P )", only printing).
+
+Notation "( 'and' a b )" := (and a b)
+  (in custom smt_expr at level 0, format "( and  a  b )").
+Notation "( 'or' a b )" := (or a b)
+  (in custom smt_expr at level 0, format "( or  a  b )").
+Notation "( 'not' P )" := (not P)
+  (in custom smt_expr at level 0, format "( not  P )").
+Notation "'true'" := True
+  (in custom smt_expr at level 0).
+Notation "'false'" := False
+  (in custom smt_expr at level 0).
+
+(*
+Notation "( 'ite' c a b )" :=
+  (match c with
+   | true => a
+   | false => b
+   end)
+  (in custom smt_expr at level 0, format "( ite  c  a  b )").
+*)
+Notation "( 'ite' c a b )" := (if c then a else b)
+  (in custom smt_expr at level 0, format "( ite  c  a  b )").
+
+
+(* Note: these are needed to compete against standard notations in order to be
+   considered at least as specific as them (which would fail if we only relied on
+   our custom function application notation) *)
+Notation "( 'not' ( = a b ) )" := (not (eq a b))
+  (in custom smt_expr at level 0, only printing,
+   format "( 'not'  ( =  a  b ) )").
+Notation "'(and'  (<=  x  y )  (<=  y  z ) )" := (and (Z.le x y) (Z.le y z))
+  (in custom smt_expr at level 0, only printing).
+Notation "'(and'  (<=  x  y )  (<  y  z ) )" := (and (Z.le x y) (Z.lt y z))
+  (in custom smt_expr at level 0, only printing).
+Notation "'(and'  (<  x  y )  (<=  y  z ) )" := (and (Z.lt x y) (Z.le y z))
+  (in custom smt_expr at level 0, only printing).
+Notation "'(and'  (<  x  y )  (<  y  z ) )" := (and (Z.lt x y) (Z.lt y z))
+  (in custom smt_expr at level 0,only printing).
+
+Notation "'(='  a  b )" := (eq a b)
+  (in custom smt_expr at level 0).
+Notation "'(<='  a  b )" := (Z.le a b)
+  (in custom smt_expr at level 0).
+Notation "'(<'  a  b )" := (Z.lt a b)
+  (in custom smt_expr at level 0).
+Notation "(-  a  b )" := (Z.sub a b)
+  (in custom smt_expr at level 0).
+Notation "(-  a )" := (Z.opp a)
+  (in custom smt_expr at level 0).
+Notation "(+  a  b )" := (Z.add a b)
+  (in custom smt_expr at level 0).
+Notation "(*  a  b )" := (Z.mul a b)
+  (in custom smt_expr at level 0).
+Notation "(pow  a  b )" := (Z.pow a b) (* NONSTANDARD *)
+  (in custom smt_expr at level 0).
+
+Notation "'(bv2int'  a )" := (word.unsigned a)
+  (in custom smt_expr at level 0).
+Notation "'((_'  'int2bv'  Width )  x )" := (@word.of_Z Width _ x)
+  (in custom smt_expr at level 0, Width constr at level 0).
+
+Notation "'(bvneg'  a )" := (word.opp a)
+  (in custom smt_expr at level 0).
+Notation "'(bvadd'  a  b )" := (word.add a b)
+  (in custom smt_expr at level 0).
+Notation "'(bvsub'  a  b )" := (word.sub a b) (* NONSTANDARD *)
+  (in custom smt_expr at level 0).
+(*
+Notation "'(bvadd'  a  '(bvneg'  b ) )" := (word.sub a b)
+  (in custom smt_expr at level 0).
+*)
+Notation "'(bvult'  a  b )" := (word.ltu a b)
+  (in custom smt_expr at level 0).
+
+Notation "( f  a )" := (f a)
+  (in custom smt_expr at level 0,
+   f custom smt_func at level 0, a custom smt_expr at level 0).
+
+Notation "( f  a1 a2 )" := (f a1 a2)
+  (in custom smt_expr at level 0,
+   f custom smt_func at level 0,
+   a1 custom smt_expr at level 0, a2 custom smt_expr at level 0).
+
+Notation "x" := (Zpos x)
+  (in custom smt_expr at level 0, x constr at level 0, only printing).
+Notation "0" := Z0
+  (in custom smt_expr at level 0, only printing).
+
+(* fallback for variables *)
+Notation "| x |" := x
+  (in custom smt_expr at level 0, x ident, only printing, format "| x |").
+
+(* Function names that are variables: *)
+Notation "| f |" := f
+  (in custom smt_func at level 0, f ident, only printing, format "| f |").
+
+
+Section Tests.
+
+(* configurable to any concrete bitwidth, so that slow bitblasting can be tested
+   with small bitwidths such as 8 *)
+Local Notation width := 7 (only parsing).
+
+Context {word: word.word width} {word_ok: word.ok word}.
+Local Open Scope word_scope.
+Local Open Scope Z_scope.
+Local Open Scope bool_scope.
+Local Hint Mode Word.Interface.word - : typeclass_instances.
+
+Add Ring wring : (Properties.word.ring_theory (word := word))
+      ((*This preprocessing is too expensive to be always run, especially if
+         we do many ring_simplify in a sequence, in which case it's sufficient
+         to run it once before the ring_simplify sequence.
+         preprocess [autorewrite with rew_word_morphism],*)
+       morphism (Properties.word.ring_morph (word := word)),
+       constants [Properties.word_cst]).
+
+Definition prelude1 := tt.
+Notation "'#!/bin/sh'" := prelude1 (only printing).
+Definition prelude2 := tt.
+Notation "'set' '-e'" := prelude2 (only printing).
+Goal True. let p1 := prelude1 in let p2 := prelude2 in idtac p1; idtac p2. Abort.
+
+Ltac t name :=
+  log_goal_as_smt name;
+  repeat standalone_solver_step.
 
 Goal forall (a b r : word) (c : bool),
  c = word.ltu a b ->
  r = (if c then a else b) -> \[a] < \[b] /\ r = a \/ \[b] <= \[a] /\ r = b.
-Proof. t. Qed.
+Proof. t name:(ltu_ite). Qed.
 
+(* TODO replace Z.min by def and support for define-fun
 Goal forall (a b c : word) (r : word),
  \[a] < \[b] /\ r = a \/ \[b] <= \[a] /\ r = b ->
  forall (s : word),
  \[r] < \[c] /\ s = r \/ \[c] <= \[r] /\ s = c ->
  \[s] = Z.min \[a] (Z.min \[b] \[c]).
-Proof. t. Qed.
+Proof. t name:(min2_1). Qed.
+*)
 
 Goal forall (l: word),
  l <> /[0] ->
  \[l] = 0 ->
  False.
-Proof. t. Qed.
+Proof. t name:(int2bv_roundtrip_contrad_0). Qed.
 
 Goal forall (l: word) (z: Z),
  l <> /[z] ->
  \[l] = z ->
  False.
-Proof. t. Qed.
+Proof. t name:(int2bv_roundtrip_contrad). Qed.
 
-Goal forall (l : list word) (lDone lTodo : list word),
- forall (x : word) (l' : list word),
- lTodo = x :: l' ->
- l = lDone ++ lTodo ->
- l = (lDone ++ [|x|]) ++ l'.
-Proof. t. Qed.
-
-Goal forall (p v : word) (t t0 : trace) (s : Z -> Prop) (res : word),
+Goal forall (p v : word) (s : Z -> Prop) (res : word),
  res = /[0] ->
  forall a : word,
  a = p ->
- t0 = t ->
- (forall x : Z, ~ s x) ->
+(* TODO forall notations!   (forall x : Z, ~ s x) -> *)
  a = /[0] ->
- \[a] = 0 - 2 ^ 32 * (0 / 2 ^ 32) ->
  ~ s \[v] ->
- (\[res] = 1 /\ s \[v] \/ \[res] = 0 /\ ~ s \[v]) /\ t0 = t.
-Proof. t. Qed.
+ (\[res] = 1 /\ s \[v] \/ \[res] = 0 /\ ~ s \[v]).
+Proof. t name:(tree_set_r1). Qed.
 
 Goal forall (fib: word -> word) (n : word),
  n <> /[0] ->
@@ -104,7 +363,8 @@ Goal forall (fib: word -> word) (n : word),
  t = a' ^+ fib i' -> b = t -> i = i' ^+ /[1] ->
  a = fib (i ^- /[1]).
 Proof.
-  t. unfold don't_know_how_to_prove. subst i. bottom_up_simpl_in_goal. reflexivity.
+  t name:(fib1).
+  unfold don't_know_how_to_prove. subst i. bottom_up_simpl_in_goal. reflexivity.
 Qed.
 
 Goal forall (fib: word -> word) (n : word),
@@ -118,7 +378,7 @@ Goal forall (fib: word -> word) (n : word),
  \[n] <= \[i] ->
  b = fib n.
 Proof.
-  t. unfold don't_know_how_to_prove. replace i with n by ZnWords. reflexivity.
+  t name:(fib2). unfold don't_know_how_to_prove. replace i with n by ZnWords. reflexivity.
 Qed.
 
 Goal forall (in0 in1 in2 : Z) (w0 : word),
@@ -127,41 +387,59 @@ Goal forall (in0 in1 in2 : Z) (w0 : word),
  c' = negb (word.ltu /[in0] /[in1]) && negb (word.ltu /[in2] /[in1]) ->
  c = negb (word.ltu /[in0] /[in2]) && negb (word.ltu /[in1] /[in2]) ->
  w2'' = (if c then /[in0] else /[in2]) ->
- 0 <= in0 < 2 ^ 32 ->
+ 0 <= in0 < 2 ^ width ->
  w1 = (if c' then /[in0] else /[in1]) ->
  w2 = (if c' then /[in2] else w2'') ->
- forall (m m0 m2 m1 m4 : mem) (c0 : bool),
+ forall (c0 : bool),
  c0 = word.ltu w2 w1 ->
- 0 <= in1 < 2 ^ 32 ->
- 0 <= in2 < 2 ^ 32 ->
+ 0 <= in1 < 2 ^ width ->
+ 0 <= in2 < 2 ^ width ->
  (if c' then in1 else if c then in2 else in0) <=
    \[if c0 then w2 else w1] <= \[if c0 then w1 else w2].
-Proof. t. Qed.
+Proof. t name:(sort3). Qed.
 
 Goal forall (v : word) (s0 : Z -> Prop) (a' : word) (res a : word) (v1 : Z),
  s0 v1 ->
- (forall x : Z, ~ (s0 x /\ x < v1)) ->
+(* (forall x : Z, ~ (s0 x /\ x < v1)) -> TODO forall, but it's not needed here *)
  res = /[0] ->
  a' <> /[0] ->
  forall here : word,
  here = /[v1] ->
  \[v] < v1 ->
- 0 <= v1 < 2 ^ 32 ->
  a = /[0] ->
  ~ (s0 \[v] /\ \[v] < v1) ->
  \[res] = 0 /\ ~ s0 \[v].
-Proof. t. Qed.
+Proof. t name:(tree_set_not_and1). Qed.
 
-Goal forall (v : word) (t : trace) (s0 : Z -> Prop) (a' : word) (res a : word) (v1 : Z),
+Goal forall (v : word) (s0 : Z -> Prop) (a' : word) (res a : word) (v1 : Z),
  s0 v1 ->
- (forall x : Z, ~ (s0 x /\ x < v1)) ->
+(* (forall x : Z, ~ (s0 x /\ x < v1)) -> TODO forall, but not actually needed here *)
  res = /[0] ->
  a' <> /[0] ->
  forall here : word,
  here = /[v1] ->
  \[v] < v1 ->
- 0 <= v1 < 2 ^ 32 ->
  a = /[0] ->
  ~ (s0 \[v] /\ \[v] < v1) ->
- (\[res] = 1 /\ s0 \[v] \/ \[res] = 0 /\ ~ s0 \[v]) /\ t = t.
+ (\[res] = 1 /\ s0 \[v] \/ \[res] = 0 /\ ~ s0 \[v]).
+Proof. t name:(tree_set_not_and2). Qed.
+
+Import ZList.List.ZIndexNotations.
+Local Open Scope zlist_scope.
+
+Ltac t ::= repeat standalone_solver_step.
+
+Goal forall (b n : word) (bs : list Z),
+ len bs = \[n] ->
+ forall (i : word),
+ \[b] < 2 ^ 8 -> i = /[0] -> List.repeatz \[b] \[i] ++ bs[\[i]:] = bs.
 Proof. t. Qed.
+
+Goal forall (l : list word) (lDone lTodo : list word),
+ forall (x : word) (l' : list word),
+ lTodo = x :: l' ->
+ l = lDone ++ lTodo ->
+ l = (lDone ++ [|x|]) ++ l'.
+Proof. t. Qed.
+
+End Tests.
